###P2.7
$\begin{aligned}G(s)=\frac{-1/sC}{R}=\frac{-1}{sCR}\end{aligned}$
***

###P2.12
$\frac{Y(s)}{R(s)}=\frac{K}{s(s+50)}$, $\begin{aligned} R(s)=\frac{1}{s}\end{aligned}$

$\begin{aligned} Y(s)=\frac{K}{s(s+50)} \end{aligned}$

=> $\begin{aligned} Y(s)=\frac{K}{50}(\frac{1}{s}-\frac{1}{s+50}) \end{aligned}$

라플라스 변환하면,
$\begin{aligned} y(t)=\frac{K}{50}(1-e^{-50t})\end{aligned}$

$\displaystyle{t\to\infty}$일 때, $\begin{aligned}y(t)=1\end{aligned}$이기 위해 $\begin{aligned} K=50\end{aligned}$
***

###P2.15
$\begin{aligned}M\frac{d^2x(t)}{dt^2}+b\frac{dx(t)}{dt}+kx(t)=v(t)\end{aligned}$

$\begin{aligned}M(s^2X(s)-sx(0^-))+b(sX(s)-x(0^-))+kX(s)=1\end{aligned}$

$\begin{aligned}Ms^2X(s)+bsX(s)+kX(s)=1\end{aligned}$

$\begin{aligned}X(s)(Ms^2+bs+k)=1\end{aligned}$

$\begin{aligned}X(s)=\frac{1}{Ms^2+bs+k}\end{aligned}$

라플라스 역변환을 하면,

$\begin{aligned}x(t)=\frac{2sin(\frac{t\sqrt{-b^2+4km}}{2m})e^{-\frac{bt}{2m}}}{\sqrt{4km-b^2}}\end{aligned}$
***

###P2.26
$\begin{aligned}F(t)-b(x'(t)-y'(t))-k(x(t)-y(t))&=Mx''(t)\end{aligned}$
$\begin{aligned}-b(y'(t)-x'(t))-k(y(t)-x(t))=my''(t)\end{aligned}$

위 두 식을 라플라스 변환하면,

$\begin{aligned}k(X(s)-Y(s))-F(s)+b(X(s)s-Y(s)s)+MX(s)s^2=0\end{aligned}$
$\begin{aligned}Y(s)ms^2-b(X(s)s-Y(s)s)-k(X(s)-Y(s))=0\end{aligned}$

위 두 식을 연립하면,

$\begin{aligned}Y(s)=\frac{F(s)(k+bs)}{s^2(bms+km+Mbs+Mk+Mms^2)}\end{aligned}$

따라서, $\begin{aligned}\frac{Y(s)}{F(s)}=\frac{k+bs}{s^2(bms+km+Mbs+Mk+Mms^2)}\end{aligned}$
***

###P2.37
$\begin{aligned}-k_1x(t)-k_2(x(t)-y(t))=m_1x''(t)\end{aligned}$
$\begin{aligned}-k_2(y(t)-x(t))-u(t)=m_2y''(t)\end{aligned}$

위 두 식이 세워지는데, $\begin{aligned}k_1=k_2=1, m_1=m_2=1\end{aligned}$이므로

$\begin{aligned}x''(t)+2x(t)-y(t)=0\end{aligned}$

$\begin{aligned}y''(t)+y(t)-x(t)+u(t)=0\end{aligned}$

라플라스 변환하면,

$\begin{aligned}X(s)s^2+2X(s)-Y(s)=0\end{aligned}$

$\begin{aligned}Y(s)s^2+U(s)-X(s)+Y(s)=0\end{aligned}$

위 두 식을 연립하면,

$\begin{aligned}Y(s)=\frac{-U(s)(s^2+2)}{s^4+3s^2+1}\end{aligned}$

따라서, $\begin{aligned}\frac{Y(s)}{U(s)}=\frac{-(s^2+2)}{s^4+3s^2+1}\end{aligned}$


```python
!jupyter nbconvert --to markdown
```
