
p2.7  

$$ \frac{-v_1}{R}+c\frac{d(-v_2)}{dt}=0$$

$$ \frac{-v_1}{R}-scV_2=0$$    

$$ v_2=\frac{-v_1}{SRC}$$  

$$ \frac{v_2(s)}{v_1(s)}=\frac{-1}{SRC}$$  

---
p2.12  
$$r(t)=unitstep$$  
$$R(s)=\frac{1}{s}$$   
$$Y(s)=\frac{k}{s+50}R(s)$$   
$$Y(s)=\frac{k}{s(s+50)}$$  

$$Y(s)=k(\frac{A}{s}+\frac{B}{s+50})$$  

$$Y(s)=k(\frac{AS+50A+BS}{s(s+50)})$$   
$$A=\frac{1}{50},
B=-\frac{1}{50}$$  
$$Y(s)=k(\frac{1}{50s}-\frac{1}{50(s+50)})$$  
$$\displaystyle\lim_{t\to\infty}y(t) = \lim_{s\to0}sY(s)=1  $$  
$$\displaystyle\lim_{t\to\infty}k(\frac{1}{50}-\frac{s}{50(s+50)})=1$$  
$$k=50$$  
$$Y(s)=\frac{1}{s}-\frac{1}{s+50}$$  
$$\displaystyle\lim_{t\to0^+}y(t) = \lim_{t\to\infty}sY(s)
=\lim_{t\to\infty}(1-\frac{s}{s+50})=0=y(0^+) $$   

---  
p2.15  
$$mx''+bx'+kx=\delta(t)$$  
$$m(s^2 X(s)-sx(0)-x'(0))+b(sX(s)-x(0))+kX(s)=1$$   
zero initial conditions(x(0)=0, x'(0)=0)  
$$ms^2 X+bsX+kX=1$$   
$$X(s)=\frac{1}{ms^2+bs+k}=\frac{1}{s^2+bs/m+k/m}
=\frac{1}{(s+b/2m)^2-b^2/4m^2+k/m}$$  
$$x(t)=\frac{sin(\sqrt(b^2/4m^2+k/m)t)e^\frac{-bt}{2m}}{\sqrt(-b^2/4m^2+k/m)} $$  

---
p2.26  
$$Mx''=f(t)-k(x-y)-b(x'-y')$$
$$my''=-k(y-x)-b(y'-x')$$

$$Mx''+bx'+kx=f(t)+by'+ky$$
$$my''+by'+ky=bx'+kx$$  
initial condition zero  
$$M(s^2 X-sx(0)-x'(0))+b(sX-x(0))+kX=F(s)+b(sY-y(0))+kY$$  
$$Ms^2 X+bsX+kX=F(s)+bsY+kY$$  
$$X(Ms^2+bs+k)=F(s)+bsY+kY$$  

$$m(s^2 Y-sy(0)-y'(0))+b(sY-y(0))+kY=b(sX-x(0))+kX$$  
$$ms^2 Y+bsY+kY=bsX+kX$$  
$$Y(ms^2+bs+k)=X(bs+k)$$  

$$X=\frac{Y(ms^2+bs+k)}{bs+k}$$를 $$X(Ms^2+bs+k)=F(s)+bsY+kY$$에 대입  
$$\frac{Y(ms^2+bs+k)}{bs+k}(Ms^2+bs+k)=F(s)+bsY+kY$$  
$$Y(\frac{(ms^2+bs+k)}{bs+k}(Ms^2+bs+k)-(bs+k))=F(s)$$  
$$\frac{Y(s)}{F(s)}=\frac{bs+k}{(ms^2+bs+k)^(Ms^2+bs+k)-(bs+k)^2}$$  

---
p2.37  
$$m_1 x''=-x(k_1+k_2)+k_2 y$$  
$$m_2 y''=k_2(x-y)-u$$  

(a) m1=m2=1, k1=k2=1  
$$x''=-2x+y$$  
$$y''=x-y-u$$  
(b)  
$$s^2 X-sx(0)-x'(0)+2X=Y$$  
$$s^2 Y-sy(0)-y'(0)+Y=X-U$$  
initial condition zero  
$$s^2 X+2X=Y$$  
$$s^2 Y+Y=X-U$$  

$$s^2 X+2X=Y$$를 $$X=\frac{Y}{s^2+2}$$로 바꿔 $$s^2 Y+Y=X-U$$ 에 대입  
$$s^2 Y+Y=\frac{Y}{s^2+2}-U$$  
$$Y=\frac{U}{\frac{1}{s^2+2}-(s^2+1)}$$

$$\frac{Y(s)}{U(s)}=\frac{1}{\frac{1}{s^2+2}-(s^2+1)}$$



```python
from google.colab import drive
drive.mount('/content/drive')
```


```python
!jupyter nbconvert --to markdown "/content/drive/MyDrive/Colab Notebooks/2단원과제"
```

    [NbConvertApp] Converting notebook /content/drive/MyDrive/Colab Notebooks/2단원과제 to markdown
    [NbConvertApp] Writing 2341 bytes to /content/drive/MyDrive/Colab Notebooks/2단원과.md

