### **P-7**
Obtain the transfer function of the integrating amplifier circuit shown in Figure P2.7, which is an implementation of a first-order low pass filter.

(1) 증폭기의 -단은 0V의 전압을 가짐으로 KCL사용하여 식을 세운다.  
(2)    $\frac{-V_1(s)}{R} = sCV_2(t)$        
(3) $G(s)=\frac{V_2(s)}{V_1(s)} = \frac{-1}{sCR}$

  
  
---
### **P-12**
For the open-loop control system described by theblock diagram shown in Figure P2.12, determine thevalue of K such that y(t)→ 1 as t → ∞ when r(t) is a unit step input. Assume zero initial conditions.  
  
(1) Y(s)의 대한 식을 세우고 최종값 정리를 이용한다.
(2) $Y(s)= \frac{k}{s+50}*R(s)$  
(3) 이때 $R(s)$는 계단 함수 임으로 라플라스 변환 시 $\frac{1}{s}$로 만들어 지고 이를 식에 대입했을 때 $Y(s)= \frac{k}{s(s+50)}$ 으로 구성된다.
(4) 최종값 정리를 이용한다.  
$1 = \displaystyle\lim_{s\rightarrow\infty}{f(t)} = \displaystyle\lim_{s\rightarrow0}{s}\frac{k}{s(s+50)}=\frac{k}{50}$
(5) 따라서 k = 50 임을 알 수 있다.

***

###**P-15**
Consider the spring-mass system depicted in Figure P2.15. Determine a differential equation to describe the motion of the mass m. Obtain the system response x(t) subjected to an impulse input with zero initial conditions.

####p-15.1  

(1) $m\frac{d^2x}{dt^2}+ b\frac{dx}{dt}+ kx(t) = 0$

####p-15.2

(1) $m\frac{d^2x}{dt^2}+ b\frac{dx}{dt}+ kx(t) = \delta(t)$
(2) $s^2X(s)+\frac{b}{m}sX(s)+\frac{k}{m}X(s) = 1$  
(3) $(s^2+\frac{b}{m}s+\frac{k}{m})X(s) = 1$
(4) $X(s) = \frac{1}{s^2+\frac{b}{m}s+\frac{k}{m}}$
(5) $\frac{2m\sin\left(\frac{t\sqrt{-b^2 + 4km}}{2m}\right)e^{-\frac{bt}{2m}}}{\sqrt{-b^2 + 4km}}$

###p-15 매트랩 코드
```matlab
syms t s b m k

Gs = 1 / (s^2 + (b/m)*s + k/m);
gt = ilaplace(Gs, s, t);

disp(gt)
```
---
###**P-26**
A robot includes significant flexibility in the arm members with a heavy load in the gripper [6, 20]. A two-mass model of the robot is shown in Figure P2.26.
Find the transfer function Y(s)/ F(s).  

(1)  $M_1 \frac{d^2x(t)}{dt^2} - k(x(t)-y(t)) - b \frac{d(x(t)-y(t))}{dt} $  
     $M_2 \frac{d^2y(t)}{dt^2} + k(x(t)-y(t)) + b \frac{d(x(t)-y(t))}{dt} $
(2) $F(s) = M_1s^2X(s)- k(X(s)-Y(s))-bs(X(s)-Y(s)) $   
    $0 = M_2s^2Y(s) + k(X(s)-Y(s)) + bs(X(s)-Y(s)) $   
    $0 = M_2s^2Y(s) + (k+bs)X(s) - (k+bs)Y(s) $   
(3) $X(s) = \frac{-M_2s^2+(k+bs)}{k+bs}Y(s) $
(4) $F(s) = M_1s^2X(s) - (k+bs)X(s) + (k+bs)Y(s)$
(5) $F(s) = k\left( Y + \frac{M2 \cdot Y \cdot s^2 - Y \cdot b \cdot s + Y \cdot k}{k + b \cdot s} \right) + b \cdot s \left( Y + \frac{M2 \cdot Y \cdot s^2 - Y \cdot b \cdot s + Y \cdot k}{k + b \cdot s} \right) - \frac{M1 \cdot s^2 \cdot (M2 \cdot Y \cdot s^2 - Y \cdot b \cdot s + Y \cdot k)}{k + b \cdot s}$
(6) $\frac{Y(s)}{F(S)} = G(s) = \frac{k + b \cdot s}{2 \cdot k^2 + 2 \cdot b \cdot k \cdot s - M1 \cdot M2 \cdot s^4 + M1 \cdot b \cdot s^3 + M2 \cdot b \cdot s^3 - M1 \cdot k \cdot s^2 + M2 \cdot k \cdot s^2} $
  

###P-26 매트랩 코드
```matlab
syms M1 M2 k b Y X F s

Ft = M1 * s^2 * X - k*(X-Y) - b*s*(X-Y);
ex0 = M2 * s^2 * Y + k*(X+Y) + b*s*(X-Y);

sol_x = solve(ex0,X);
F_s = subs(Ft, X, sol_x);

%disp(F_s);
disp(simplify(Y/F_s));
```
***

###**P-37**
A two-mass system is shown in Figure P2.37 with an input force u(t). When m1 = m2 = 1 and K1 = K2 = 1, (a) find the set of differential equations describing the system, and (b) compute the transfer function from U(s) to Y(s).  

####P-37.1
(1)  $M_1\frac{d^2x(t)}{dt^2} - k_1(x(t)-y(t)) - k_2(x(t)-y(t)) + u(t) = 0 $  
(2) $M_2\frac{d^2y(t)}{dt^2} =  k_2(x(t)-y(t))$  

####P-37.2
(1)$M_2s^2Y(s) = k_2(X(s)-Y(s))$  
(2)$\frac{M_2s^2+k_2}{k_2}Y(s)= X(s)$  
(3)$M_1s^2X(s) = -(k_1+k_2)X(s)+k_2Y(s) +U(s)$  
(4)$(M_1s^2+k_1+k_2)\frac{M_2s^2+k_2}{k_2}Y(s)-k_2Y(s)=U(s)$  
(5)$((M_1s^2+k_1+k_2)\frac{M_2s^2+k_2}{k_2}-k_2)Y(s)=U(s)$  
(6)$\frac{Y(s)}{U(s)} =\frac{1}{((M_1s^2+k_1+k_2)\frac{M_2s^2+k_2}{k_2}-k_2)}$  
(7) $k_1,k_2,M_1,M_2$ 값인 1을 대입  
   $\frac{Y(s)}{U(s)} = \frac{1}{s^4+3s^2+1}$

###P-37 매트랩 코드

```matlab
clear;
syms s X Y U

m1 = 1;
m2 = 1;
K1 = 1;
K2 = 1;

eq1 = m1 * X * s^2 + K1 * X - K2 * (Y - X) - U;
eq2 = m2 * Y * s^2 - K2 * (X - Y);

solutions = solve([eq1, eq2], [Y, U]);

G = simplify(solutions.Y / solutions.U);

disp(G);


```
